LeanPy/Data/Tuple/Basic.lean
@@ -1,0 +1,54 @@
+/-
+Copyright (c) 2025 Mac Malone. All rights reserved.
+Released under the Apache 2.0 license as described in the file LICENSE.
+Authors: Mac Malone
+-/
+import LeanPy.Data.Object.Slots
+
+namespace LeanPy
+
+/-- A pure Python tuple. -/
+abbrev Tuple := Array Object
+
+namespace Tuple
+
+/-- Returns the hash of the tuple. -/
+-- Should follow the logic in CPython's `tuplehash`
+-- https://github.com/python/cpython/blob/3.11/Objects/tupleobject.c#L321
+-- adjusted to Lean's hashing algorithm (but maybe should use CPython's?)
+def hashM (self : Tuple) : PyM Hash := do
+  let baseHash := 7 -- base hash used by `Array`
+  self.foldlM (init := baseHash) fun hash obj => do
+    return mixHash hash (← obj.hashM)
+
+/--
+Returns `true` if the two tuples are equal.
+
+Tuples compare equal if and only if their elements compare equal.
+-/
+-- Should follow the logic in CPython's `tuplerichcompare`
+-- https://github.com/python/cpython/blob/3.11/Objects/tupleobject.c#L628
+def beqM (self other : Tuple) : PyM Bool := do
+  if h : self.size = other.size then
+    self.size.anyM fun i h => self[i].beqM other[i]
+  else
+    return false
+
+/--
+Returns a string representation of the tuple.
+
+Tuples compare equal if and only if their elements compare equal.
+-/
+-- Should follow the logic in CPython's `tuplerepr`
+-- https://github.com/python/cpython/blob/3.11/Objects/tupleobject.c#L219
+def reprM (self : Tuple) : PyM String := do
+  -- NOTE: CPython does a recursion check here, but likely we don't need it?
+  if h0 : self.size = 0 then
+    return "()"
+  else if h1 : self.size = 1 then
+    return s!"({← self[0].reprM},)"
+  else
+    let init := s!"({← self[0].reprM}, {← self[1].reprM}"
+    let s ← self.foldlM (init := init) (start := 2) fun s obj =>
+      return s!"{s}, {← obj.reprM}"
+    return s.push ')'
