LeanPy/Data/Tuple/Object.lean
@@ -1,0 +1,132 @@
+/-
+Copyright (c) 2025 Mac Malone. All rights reserved.
+Released under the Apache 2.0 license as described in the file LICENSE.
+Authors: Mac Malone
+-/
+import LeanPy.Data.Tuple.Ref
+import LeanPy.Data.Object.Slots
+import LeanPy.Data.Str.Object
+
+namespace LeanPy
+
+/- An instance of a subclass of `tuple` that satisfies `p`. -/
+abbrev PTupleObject (p : ObjectProp) := PSubObject p tupleTypeRef
+
+/- An instance of a subclass of `tuple`. -/
+def TupleObject := PTupleObject .Any
+
+/-- Returns whether this object is an instance of a subtype of `tuple`. -/
+@[inline] def Object.isTuple (self : Object) : Bool :=
+ self.ty.isTupleSubclass
+
+/-- Casts `self` to `TupleObject`. -/
+@[inline] def Object.asTuple (self : Object) (h : self.isTuple) : TupleObject :=
+  self.asSubObject (self.ty.isTupleSubclass_iff_subset.mp h)
+
+/--
+Casts `self` to `TupleObject` if `self` is instance of a subtype of `tuple`.
+Otherwise, returns `none`.
+-/
+@[inline] def Object.asTuple? (self : Object) : Option TupleObject :=
+  if h : self.isTuple then some (self.asTuple h) else none
+
+namespace ObjectData
+
+@[inline] private unsafe def ofTupleRefImpl (tuple : TupleRef) : ObjectData :=
+  unsafeCast tuple
+
+@[implemented_by ofTupleRefImpl]
+abbrev ofTupleRef (tuple : TupleRef) : ObjectData := .mkCore tupleDataKind tuple
+
+opaque getTupleRef (self : ObjectData) (h : self.kind = tupleDataKind) : TupleRef :=
+  unsafe unsafeCast self
+
+end ObjectData
+
+namespace TupleObject
+
+instance : Coe TupleObject Object := ⟨PObject.toObject⟩
+
+theorem isTuple_toObject (self : TupleObject) : self.toObject.isTuple :=
+  self.ty.isTupleSubclass_iff_subset.mpr self.ty_subset
+
+@[inline] def getTupleRef (self : TupleObject) : TupleRef :=
+  self.data.getTupleRef (self.lawful_subobject).2
+
+@[inline] def getTuple (self : TupleObject) : Tuple :=
+  self.getTupleRef.data
+
+/--
+Returns the hash of the tuple.
+
+This is equivalent to the Python `tuple.__hash__(self)`.
+-/
+@[inline] protected def hashM (self : TupleObject) : PyM Hash :=
+  self.getTuple.hashM
+
+
+/--
+Returns `true` if the two tuples are equal.
+
+This is equivalent to the Python `tuple.__eq__(self, other)`.
+-/
+@[inline] protected def beqM (self other : TupleObject) : PyM Bool :=
+  self.getTuple.beqM other.getTuple
+
+/--
+Returns `true` if the two tuples are not equal.
+
+This is equivalent to the Python `tuple.__ne__(self, other)`.
+-/
+@[inline] protected def bneM (self other : TupleObject) : PyM Bool :=
+  not <$> self.beqM other
+
+/--
+Return the number of items in the tuple.
+
+This is equivalent to the Python `tuple.len(self)`.
+-/
+@[inline] def length (self : TupleObject) : Nat :=
+  self.getTuple.size
+
+/-- Return `true` unless the tuple is empty. -/
+@[inline] def toBool (self : TupleObject) : Bool :=
+  self.length != 0
+
+/--
+Return a string representation of the tuple.
+
+This is equivalent to the Python `tuple.__repr__(self)`.
+-/
+@[inline] def reprM (self : TupleObject) : PyM String :=
+  self.getTuple.reprM
+
+end TupleObject
+
+def tupleTypeRef.slots : TObjectSlots TupleObject where
+  hash self := self.hashM
+  beq self other :=
+    if let some other := other.asTuple? then self.beqM other else return false
+  bne self other :=
+    if let some other := other.asTuple? then self.bneM other else return true
+  bool self := return self.toBool
+  repr self := self.reprM
+
+@[instance] initialize tupleTypeSlotsRef : TypeSlots tupleTypeRef ←
+  tupleTypeRef.slots.mkRef
+
+namespace TupleObject
+
+@[inline] def ofTupleRef (r : TupleRef) : TupleObject :=
+  tupleTypeRef.mkObjectCore r.id  (.ofTupleRef r)
+
+instance : Coe TupleRef TupleObject := ⟨TupleObject.ofTupleRef⟩
+
+def empty : TupleObject := .ofTupleRef .empty
+
+instance : EmptyCollection TupleObject := ⟨TupleObject.empty⟩
+
+end TupleObject
+
+@[inline] def mkTupleObject (data : Array Object) : BaseIO TupleObject :=
+  .ofTupleRef <$> mkTupleRef data
