LeanPy/Data/Tuple/Ref.lean
@@ -1,0 +1,30 @@
+/-
+Copyright (c) 2025 Mac Malone. All rights reserved.
+Released under the Apache 2.0 license as described in the file LICENSE.
+Authors: Mac Malone
+-/
+import LeanPy.Data.Tuple.Basic
+
+namespace LeanPy
+
+/- An immutable reference to a tuple. -/
+abbrev TupleRef := NonScalarRef Tuple
+
+instance : Nonempty {r : TupleRef // r.data = data} :=
+  ⟨NonScalarRef.null data, NonScalarRef.data_null⟩
+
+@[inline] opaque mkTupleRef' (data : Tuple) : BaseIO {r : TupleRef // r.data = data} :=
+  pure (unsafe unsafeCast data)
+
+@[inline] def mkTupleRef (data : Tuple) : BaseIO TupleRef := do
+  Subtype.val <$> mkTupleRef' data
+
+namespace TupleRef
+
+initialize empty' : {r : TupleRef // r.data = #[]} ← mkTupleRef' _
+
+@[inline] def empty : TupleRef := empty'.val
+
+@[simp] theorem data_empty : empty.data = #[] := empty'.property
+
+instance : EmptyCollection TupleRef := ⟨TupleRef.empty⟩
