LeanPy/Data/Tuple/TypeRef.lean
@@ -1,0 +1,30 @@
+/-
+Copyright (c) 2025 Mac Malone. All rights reserved.
+Released under the Apache 2.0 license as described in the file LICENSE.
+Authors: Mac Malone
+-/
+import LeanPy.Data.Object.TypeRef
+
+namespace LeanPy
+
+def tupleType.doc : String := "\
+  Built-in immutable sequence.\n\
+  \n\
+  If no argument is given, the constructor returns an empty tuple.\n\
+  If iterable is specified the tuple is initialized from iterable's items.\n\
+  \n\
+  If the argument is a tuple, the return value is the same object.\
+  "
+
+def tupleDataKind : DataKind := `LeanPy.TupleRef
+
+@[reducible] def tupleType : PyType where
+  name := "tuple"
+  doc? := some tupleType.doc
+  base? := some objectTypeRef
+  isTupleSubclass := true
+  IsValidObject id data := id.isNonScalar ∧ data.kind = tupleDataKind
+
+initialize tupleTypeRef.init : InitTypeRef tupleType ← initTypeRef
+
+abbrev tupleTypeRef : TypeRef := tupleTypeRef.init.toTypeRef
